compcert_new/cfrontend/Clight.v
@@ -493,51 +493,6 @@ Inductive state: Type :=
       (k: cont)
       (m: mem) : state.
 
-(**NEW *)
-Definition get_mem (s:state):=
-  match s with
-  | State _ _ _ _ _ m => m
-  | Callstate _ _ _ m => m
-  | Returnstate _ _ m => m
-  end.
-
-(**NEW *)
-Definition set_mem (s:state)(m:mem):=
-  match s with
-  | State f s k e le _ => State f s k e le m
-  | Callstate fd args k _ => Callstate fd args k m
-  | Returnstate res k _ => Returnstate res k m
-  end.
-
-(**NEW *)
-Definition at_external (c: state) : option (external_function * list val) :=
-  match c with
-  | State _ _ _ _ _ _ => None
-  | Callstate fd args k _ =>
-      match fd with
-        Internal f => None
-      | External ef targs tres cc => 
-          Some (ef, args)
-      end
-  | Returnstate _ _ _ => None
- end.
-
-(**NEW *)
-Definition after_external (rv: option val) (c: state) (m0:mem): option state :=
-  match c with
-     Callstate fd vargs k m =>
-        match fd with
-          Internal _ => None
-        | External ef tps tp cc =>
-            match rv with
-              Some v => Some(Returnstate v k m0)
-            | None  => Some(Returnstate Vundef k m0)
-            end
-        end
-   | _ => None
-  end.
-
-
 (** Find the statement and manufacture the continuation
   corresponding to a label *)
 
@@ -714,17 +669,6 @@ Inductive step: state -> trace -> state -> Prop :=
   corresponding to the invocation of the ``main'' function of the program
   without arguments and with an empty continuation. *)
 
-
-(*Inductive entry_point (p: program): mem -> state -> val -> list val -> Prop :=
-  | entry_point_intro: forall b f args m0,
-      let ge := Genv.globalenv p in
-      Genv.init_mem p = Some m0 ->
-      Genv.find_symbol ge p.(prog_main) = Some b ->
-      Genv.find_funct_ptr ge b = Some f ->
-      type_of_fundef f = Tfunction Tnil type_int32s cc_default ->
-      entry_point p m0 (Callstate f nil Kstop m0) (Vptr b Ptrofs.zero) args.*)
-
-
 Inductive initial_state (p: program): state -> Prop :=
   | initial_state_intro: forall b f m0,
       let ge := Genv.globalenv p in
@@ -734,57 +678,8 @@ Inductive initial_state (p: program): state -> Prop :=
       type_of_fundef f = Tfunction Tnil type_int32s cc_default ->
       initial_state p (Callstate f nil Kstop m0).
 
-(*NEW*)
-(* The following parameters are simple and reasonable, *)
-(* but might not be needed. All definitions come from  *)
-(* compcomp/core/val_casted.v                          *)
-
-(*Parameter val_casted_list_func: list val -> typelist -> bool. (* TODO *)
-Parameter tys_nonvoid: typelist -> bool .
-Parameter vals_defined: list val -> bool.
- *)
-
-(* No unvalid pointers, i.e. othing pointing after nextblock *)      
-Definition mem_well_formed m:=
-  Mem.inject (Mem.flat_inj (Mem.nextblock m)) m m.
-
-(* All arguments are in memory and without unvalid pointers*)
-Definition arg_well_formed args m0:=
-      Val.inject_list (Mem.flat_inj (Mem.nextblock m0)) args args.
-
-Inductive val_casted_list: list val -> typelist -> Prop :=
-  | vcl_nil:
-      val_casted_list nil Tnil
-  | vcl_cons: forall v1 vl ty1 tyl,
-      val_casted v1 ty1 -> val_casted_list vl tyl ->
-      val_casted_list (v1 :: vl) (Tcons  ty1 tyl).
-
-(* Require Import Conventions.
-
-Definition loc_arguments' l := if Archi.ptr64 then loc_arguments_64 l 0 0 0 else loc_arguments_32 l 0. *)
-
-(*NOTE: DOUBLE CHECK TARGS (it's not used right now)*)
-Inductive entry_point (ge:genv): mem -> state -> val -> list val -> Prop :=
-| initi_core:
-    forall f fb b0 f0 m0 m1 stk args targs tres,
-      Genv.find_funct_ptr ge fb = Some f ->
-      type_of_fundef f = Tfunction targs tres cc_default ->
-      globals_not_fresh ge m0 ->
-      Mem.mem_wd m0 ->
-      Mem.arg_well_formed args m0 ->
-      val_casted_list args targs ->
-      Val.has_type_list args (typlist_of_typelist targs) ->
-      (*val_casted_list_func args targs 
-                           && tys_nonvoid targs 
-                           && vals_defined args
-                           && zlt (4*(2*(Zlength args))) Int.max_unsigned = true ->*)
-      Genv.find_funct_ptr ge b0 = Some (Internal f0) ->
-      Mem.alloc m0 0 0 = (m1, stk) ->
-      entry_point ge m0 (Callstate f args (Kcall None f0 empty_env
-                                                 (temp_bindings
-                                                    1%positive (Vptr fb Ptrofs.zero::args)) Kstop) m1) (Vptr fb Ptrofs.zero) args.
-
 (** A final state is a [Returnstate] with an empty continuation. *)
+
 Inductive final_state: state -> int -> Prop :=
   | final_state_intro: forall r m,
       final_state (Returnstate (Vint r) Kstop m) r.
@@ -818,32 +713,13 @@ Definition step2 (ge: genv) := step ge (function_entry2 ge).
 
 (** Wrapping up these definitions in two small-step semantics. *)
 
-Definition part_semantics1 (ge: genv) :=
-  Build_part_semantics get_mem set_mem (step1 ge)
-                       (entry_point ge)
-                       at_external
-                       after_external
-                       final_state ge ge.
-
 Definition semantics1 (p: program) :=
   let ge := globalenv p in
-  let main :=Genv.find_symbol ge p.(prog_main) in
-  let init_mem:=(Genv.init_mem p) in
-  Build_semantics (part_semantics1 ge) main init_mem.
-
-Definition part_semantics2 (ge: genv) :=
-  Build_part_semantics get_mem set_mem (step2 ge)
-                       (entry_point ge)
-                       at_external
-                       after_external
-                       final_state ge ge.
+  Semantics_gen step1 (initial_state p) final_state ge ge.
 
 Definition semantics2 (p: program) :=
   let ge := globalenv p in
-  let main :=Genv.find_symbol ge p.(prog_main) in
-  let init_mem:=(Genv.init_mem p) in
-  Build_semantics (part_semantics2 ge) main init_mem.
-
+  Semantics_gen step2 (initial_state p) final_state ge ge.
 
 (** This semantics is receptive to changes in events. *)
 
